\documentclass{article}
\usepackage{tbil-de}
\usepackage[top=1in,bottom=1in,right=1in,left=1in]{geometry}

\parindent=0pt

%Problem environment -- takes an argument which is the standard
\newenvironment{problem}[1]
%before
{
  \begin{flushleft}
  %{\bfseries \arabic{problem} .}
  %Problem numbering by standard
  \textbf{#1}.
  \ignorespaces
}
%after
{
  \end{flushleft}
}

\newenvironment{solution}
%before
{
  \ignorespaces
  \textbf{Solution:}
}
%after
{
  \ignorespacesafterend
  \begin{flushright}
  {\bfseries \qed}
  \end{flushright}
}



\begin{document}

\begin{center}
\Large \textbf{Sample Assessment Exercises}
\end{center}

This document contains one exercise and solution for each standard.
The goal is to give you an idea of what the exercises might look like,
and what the expectations for a complete solution are.

\begin{problem}{C1}
Find the general solution to \[y'+y=-t^2.\]
\end{problem}
\begin{solution}
First, we find a general solution to the homogeneous equation \[y'+y=0.\]  This has auxilliary equation \(r+1=0\), which has a single root at \(r=1\), so \(ce^{-t}\) is a solution.  We can find a particular solution \(y_p\) to the given equation by using undetermined coefficients; since \(-t^2\) is a polynomial, we let \(y_p = At^2+Bt+D\) and determine the coefficients \(A\), \(B\), and \(D\).  
\begin{align*}
y_p ^\prime +y_p= &= (2At+B)+(At^2+Bt+D) \\
&= At^2+(2A+B)+(B+D)
\end{align*}

So if \(y_p\) is a solution, we must have \(y_p ^\prime+y_p = -t^2\), giving us the system of equations
\begin{align*}
A&=-1 \\ 2A+B &= 0 \\ B+D&=0
\end{align*}
Thus we easily deduce that \(A=-1\), \(B=2\), and \(D=-2\), giving \(y_p = -t^2+2t-2\).  Thus, the general solution is
\[y = -t^2+2t-2+ce^{-t}.\]
\end{solution}


\begin{problem}{C2}
Consider the following scenario: 
A water droplet with a radius of \(10\ {\rm \mu m}\) has a mass of about \(4 \times 10^{-15} {\rm kg}\) and a terminal velocity of \(3\ {\rm \frac{cm}{s}}\).  The droplet is dropped from rest.  
\begin{enumerate}[(a)]
\item Write down an IVP modelling the velocity of the water droplet.
\item What is its velocity after \(0.01\ {\rm s}\)?
\end{enumerate}
\end{problem}
\begin{solution}
The forces acting on the water droplet are gravity (\(mg\) downwards) and air resistance; in a water droplet this size, this is proportional to its velocity.  Let \(b\) denote this drag coefficient; then by Newton's second law (if we let up be the positive direction and down be negative), we have
\[ m \frac{dv}{dt} = -mg - bv .\]
Note that we have \(-mg\) since gravity always acts downwards, and \(-bv\) because the drag acts in the opposite direction of \(v\).
It is actually convenient to let \(a=\frac{b}{m}\), and divide this equation by the mass, yielding 
\[ \frac{dv}{dt} = -g - av .\]
This is a separable differential equation; we thus have
\[ \int \frac{1}{g+av}\ dv = \int (-1)dt .\]
Thus, \(\frac{1}{a}\ln|g+av| = -t+c_1\), or \(|g+av| = e^{-at+ac_1}=c_2e^{-at}\) (where \(c_2=e^{ac_1}\)).  To avoid the pesky absolute value sign, we can absorb a potential negative into the constant to write \(g+av=c_3 e^{-at}\), or (letting \(c_0=\frac{c_3}{a}\))
\[ v=-\frac{g}{a} +c_0 e^{-at}.\]
Note that \(\lim _{t \rightarrow \infty} v = -\frac{g}{a}\), so since we are given the terminal velocity, so after converting to meters per second we can solve \(-0.03 = -\frac{9.8}{a}\) to obtain \(a=\frac{9.8}{0.03}\).  We also know that it is dropped from rest, so we compute \(0=v(0)=-0.03+c_0\), so \(c_0=0.03\).  Thus our model for velocity is 
\[ v=-0.03+0.03e^{-\frac{9.8}{0.03} t}.\]
Then we simply compute \(v(0.01)=-0.03+0.03e^{-\frac{9.8}{0.03} (0.01)} \approx -0.029 \).  So after \(0.01\ {\rm s}\), the drop is falling approximately  \(2.9\ {\rm \frac{cm}{s}}\).
\end{solution}


\begin{problem}{C3}
Find the general solution to \[y''+6y'+13y=0.\]
\end{problem}
\begin{solution}
We begin by writing the auxilliary equation \(r^2+6r+13=0\) and finding the roots.  There are many ways to do this; here, we complete  the square:
\[0=r^2+6r+13=r^2+6r+9+4=(r+3)^2+4.\]
Thus, we can easily solve to obtain \(r=-3\pm2i\).  Thus the general solution is
\[ y= c_1 e^{-3t} \cos(2t) + c_2 e^{-3t} \sin(2t) .\]
\end{solution}

\begin{problem}{C4}
Find the solution to
\[
y'' + 10y' + 24y = 0
\]
when \(y(0)=-3\) and \(y'(0)=2\).
\end{problem}
\begin{solution}
The auxilliary equation is \(r^2+10r+24=0\), which has roots \(r=-6\) and \(r=-4\).  Thus, the general solution is of the form \(y=c_1e^{-4t}+c_2e^{-6t}\).  
\begin{align*}
-3 &= y(0) = c_1+c_2 \\
2 &= y'(0)  = -4c_1-6c_2 
\end{align*}
Solving this system yields \(c_1 =-8\) and \(c_2 = 5\), so the solution to the IVP is \[y=-8e^{-4t}+5e^{-6t}\]
\end{solution}



\begin{problem}{C5}
Find the general solution to \[y''+6y'+13y=13t^2-t-4.\]
\end{problem}
\begin{solution}
First, we find a general solution to the homogenous equation \(y''+6y'+13y=0\).  We begin by writing the auxilliary equation \(r^2+6r+13=0\) and finding the roots.  There are many ways to do this; here, we complete  the square:
\[0=r^2+6r+13=r^2+6r+9+4=(r+3)^2+4.\]
Thus, we can easily solve to obtain \(r=-3\pm2i\).  Thus the general solution to the homogeneous equation is
\[ y= c_1 e^{-3t} \cos(2t) + c_2 e^{-3t} \sin(2t) .\]
To find a particular solution to  \(y''+6y'+13y=13t^2-t-4\), we set \(y_p=At^2+Bt+D\) and determine the coefficients \(A,B,D\).  
\begin{align*}
y_p ^{\prime\ \prime}+6y_p ^\prime +13y_p &= (2A)+6(2At+B)+13(At^2+Bt+D) \\
&= (13A)t^2 + (12A+13B)t+(2A+6B+13D)
\end{align*}
This gives us the system of equations
\begin{align*}
13A &= 13 \\
12A+13B &= -1 \\
2A+6B+13D &= -4
\end{align*}
Then we easily deduce \(A=1\), \(B=-1\), and \(D=0\), so that \(y_p = t^2-t\).  Thus, the general solution to the nonhomogeneous equation is \[y= c_1 e^{-3t} \cos(2t) + c_2 e^{-3t} \sin(2t) +t^2-t .\]

\end{solution}


\begin{problem}{C6}
Consider the following scenario:
A \(2 {\rm kg}\) mass is suspended by a spring (with spring constant \(8 {\rm kg /s^2}\)).  The mass is pulled down \(1 {\rm m}\) from its equillibrium position and released from rest.  
\begin{enumerate}[(a)]
\item Write down an IVP modelling the position of the mass.
\item How long does it take for the mass to return to its equillibrium point?
\end{enumerate}
\end{problem}
\begin{solution}
Let \(y\) denote the vertical distance from equillibrium; then the forces acting are gravity and the spring force, giving the ODE
\[ 2y''+8y=0 .\]
Simplifying, we have \(y''+4y=0\), so the general solution is \(y=c_1 \cos(2t)+c_2\sin(2t)\).  The initial conditions are \(y(0)=-1\) and \(y'(0)=0\), which imply \(c_1=-1\) and \(c_2=0\), so the system is modelled by \(y=-\cos(2t)\).  This is first zero when \(2t=\frac{\pi}{2}\), i.e. when \(t=\frac{\pi}{4}\).  Thus the mass takes \(\frac{\pi}{4}\) {\rm s} to return to its equillibrium point.
\end{solution}




\begin{problem}{F1}
Sketch a solution curve through each point marked in the slope field.

\begin{center}\begin{tikzpicture}
    \begin{axis}[
        title={\(y' = -y -x^2 \)},
        domain=-3:3,
        view={0}{90},
        axis background/.style={fill=white},
    ]
        \addplot3[black,
            quiver={
             u={1/(sqrt(1 + (-y -x*x)^2))},
             v={(-y - x*x)/(sqrt(1 + (-y - x*x)^2))},
             scale arrows=0.2,
            },
            -stealth,samples=15]
                {exp(-x) - 1/2*sin(x) - 1/2*cos(x)};
        %KAWWWWWWW
        % Here be some points added to the swoopy loop vector fieldamagigs
        \addplot[mark=*] coordinates {(-1,2)}; % Obvious ordered pair for lococation
        \addplot[mark=*] coordinates {(-1,-2)};
    \end{axis}
\end{tikzpicture}\end{center}
\end{problem}


\begin{solution}

\begin{center}\begin{tikzpicture}
    \begin{axis}[
        title={\(y' = -y - x^2\)},
        domain=-3:3,
        view={0}{90},
        axis background/.style={fill=white},
    ]
        \addplot3[black,
            quiver={
             u={1/(sqrt(1 + (-y -x*x)^2))},
             v={(-y - x*x)/(sqrt(1 + (-y - x*x)^2))},
             scale arrows=0.2,
            },
            -stealth,samples=15]
                {exp(-x) - 1/2*sin(x) - 1/2*cos(x)};
        %KAWWWWWWW
        % Here be some points added to the swoopy loop vector fieldamagigs
        \addplot[mark=*] coordinates {(-1,2)}; % Obvious ordered pair for lococation
		\addplot[red,domain=-1.25:2.5] {-x^2+2*x-2+7/exp(1)*exp(-x)};
        \addplot[mark=*] coordinates {(-1,-2)};
		\addplot[red,domain=-2.82:2.5] {-x^2+2*x-2+3/exp(1)*exp(-x)};
    \end{axis}
\end{tikzpicture}\end{center}
\end{solution}


\begin{problem}{F2}
Solve \(y'+xy=x\).
\end{problem}
\begin{solution}
Rearranging, we have \(y'=x-xy=x(1-y)\), so we see the equation is separable, and write
\[ \frac{y'}{1-y} = x .\]

Thus we compute \(\int \frac{y'}{1-y}\ dx = \int \frac{1}{1-y}\ dy = -\ln|1-y|+c_1\), and \(\int x\ dx = \frac{1}{2}x^2+c_2\).  
Thus, we have (letting \(c_3=c_2-c_1\)) \[-\ln|1-y|=\frac{1}{2}x^2+c_3.\]
Then exponentiating, we have (letting \(c_4=\pm e^{-c_3}\) ) \(1-y=c_4e^{-\frac{1}{2}x^2}\), so (with \(c=-c_4\) ) the general solution is   \[y=1+c e^{-\frac{1}{2}x^2}.\]
\end{solution}

\begin{problem}{F3}

\end{problem}
\begin{solution}

\end{solution}



\begin{problem}{F4}
Consider the autonomous equation 
\[\frac{dx}{dt} = x^2-1.\]  
\begin{enumerate}[(a)]
\item Find and classify the critical points.
\item Describe the long term behavior of the solution passing through the point \( x(4)=0 \).
\end{enumerate}
\end{problem}
\begin{solution}

Note that \(x^2-1=(x-1)(x+1)\), so there are equillibria solutions at \(x=1\) and \(x=-1\).  We can thus compute a number line for \(x'\):

\begin{center}
\begin{tikzpicture}
\node at (-3.5,0) {\(x'\)};
\draw[<->] (-3,0) -- (3,0);
\node at (-2,0.3) {\(+\)};
\node at (0,0.3) {\(-\)};
\node at (2,0.3) {\(+\)};
\draw[thick,blue] (-1,-0.2) -- (-1,0.2);
\node at (-1,-0.4) {\(-1\)};
\draw[thick,blue] (1,-0.2) -- (1,0.2);
\node at (1,-0.4) {\(1\)};
\node[red] at (-1.5,0) {\(>>>\)};
\node[red] at (-0.5,0) {\(<<<\)};
\node[red] at (0.5,0) {\(<<<\)};
\node[red] at (1.5,0) {\(>>>\)};
\node[fill,circle,green,scale=0.5] at (0,0) {};
\end{tikzpicture}
\end{center}

We see that \(-1\) is a sink (stable), while \(1\) is a source (unstable).  A trajectory passing through \(x(4)=0\) will approach \(x=-1\) in the limit.
\end{solution}

\begin{problem}{F5}
Solve \(y'+xy=x^3\).
\end{problem}
\begin{solution}
Solve homog; then variation of parameters.
\end{solution}

\begin{problem}{F6}
One of the two ODEs below is exact.  Identify which one, and solve it.
\begin{align*}
 (x + 3y)y'+y &=3x \\ %Exact
 (x + 3y)y'-y &=-3x  
\end{align*}
\end{problem}
\begin{solution}
Rewrite the first equation as \(y'=\frac{3x-y}{x+3y}\); this corresponds to the autonomous system 
\begin{align*}
\frac{dy}{dt} &= 3x - y \\
\frac{dx}{dt} &= x + 3y 
\end{align*}
If there is a function with \(\nabla F = \langle -(3x-y), x+3y\rangle\), then \[\frac{d}{dt}F(x,y)=\frac{\partial F}{\partial x} \frac{\partial x}{\partial t} + \frac{\partial F}{\partial y} \frac{\partial y}{\partial t} = -(3x-y)(x+3y)+(x+3y)(3x-y)=0\], so \(F(x,y)=c\) is a solution of the autonomous system.

Note that  \(\langle -(3x-y), x+3y\rangle\) is conservative, as \(\frac{\partial}{\partial x}(x+3y)=1=\frac{\partial}{\partial y}(-3x+y)\); so a potential function \(F\) is found by integrating: \(F = \int x+3y\ dy = xy+\frac{3}{2}y^2+f(x) \), and differentiating with respect to \(x\), we have \(-3x+y=y+f'(x)\), so \(f'(x)=-3x\), in which case \(f(x)=\int -3x\ dx = \frac{-3}{2}x^2\), so a potential function is \(F(x,y)=xy+\frac{3}{2}y^2-\frac{3}{2}x^2\).  So the general solution to the ODE is
\[ xy+\frac{3}{2}y^2-\frac{3}{2}x^2 = c.\]
\end{solution}


\begin{problem}{S1}

\end{problem}
\begin{solution}

\end{solution}

\begin{problem}{S2}

\end{problem}
\begin{solution}

\end{solution}

\begin{problem}{S3}

\end{problem}
\begin{solution}

\end{solution}


\begin{problem}{N1}

\end{problem}
\begin{solution}

\end{solution}

\begin{problem}{N2}

\end{problem}
\begin{solution}

\end{solution}

\begin{problem}{N3}

\end{problem}
\begin{solution}

\end{solution}

\begin{problem}{N4}

\end{problem}
\begin{solution}

\end{solution}

\begin{problem}{N5}

\end{problem}
\begin{solution}

\end{solution}


\begin{problem}{D1}

\end{problem}
\begin{solution}

\end{solution}

\begin{problem}{D2}

\end{problem}
\begin{solution}

\end{solution}

\begin{problem}{D3}

\end{problem}
\begin{solution}

\end{solution}

\begin{problem}{D4}

\end{problem}
\begin{solution}

\end{solution}



\end{document}
