%!TEX root =../../../course-notes.tex
% ^ leave for LaTeXTools build functionality

\begin{applicationActivities}

\begin{activity}{10}
Solve the ODE \[ y''-4y'+4y=0.\]
\end{activity}

\begin{observation}
To solve this, we need to find the kernel of \( (D-2I)(D-2I) \).
\begin{itemize}
\item The kernel of \(D-2I\) is \(\left\{ ce^{2t}\ \middle|\ c \in \IR \right\}\).
\item However, if \( (D-2I)(y) = Ae^{2t} \), then applying \(D-2I\) twice will yield zero.
\item So we must solve the ODE \[y'-2y=e^{2t}.\]
\end{itemize}

We thus turn our attention to \term{non-homogeneous} first order constant coefficent ODEs.
\end{observation}


\begin{observation}
To solve \(y'-2y=e^{2t}\), we set \(\L=D-2I\), so that we are trying to solve \[\L(y)=e^{2t}.\]  
Note that if \(y_p\) and \(y_q\) are two solutions, then \[\L(y_p-y_q)=\L(y_p)-\L(y_q)=e^{2t}-e^{2t}=0.\]
That is, \(y_p-y_q\) is a solution of the \textbf{homogeneous} ODE \(\L(y)=0\).

So if we know the general solution of \(\L(y)=0\), and a single solution of \(\L(y)=e^{2t}\), we have the general solution of \(\L(y)=e^{2t}\).
\end{observation}

\begin{activity}{15}
Suppose we have found  \(y(t)\) is a solution of \(\L(y)=0\), we will use \term{variation of parameters} and suppose a solution of \(\L(y_p)=e^{2t}\) is of the form \[y_p =v(t) y(t)\].  If we can deduce what \(v(t)\) is, we will be done.
\begin{subactivity}
Compute \(\L(vy)\) (recall \(\L=D-2I\)).
\end{subactivity}
\begin{subactivity}
Set \(\L(vy)=e^{2t}\); substituting in \(y=e^{2t}\), solve \(v'y=e^{2t}\) to find \(v\).  
\end{subactivity}
\begin{subactivity}
Write the general solution of \(y'-2y=e^{2t}\).
\end{subactivity}
\end{activity}

\begin{observation}
Thus, we have shown that the general solution of \(y''-4y'+4y=e^{2t}\) is \(c_0e^{2t}+c_1te^{2t}\).
\end{observation}

\begin{activity}{15}
Find the general solution to \(y'-y=e^{3t}\).
\begin{subactivity}
First, solve the homogeneous equation \(\L(y)=0\).
\end{subactivity}
\begin{subactivity}
Set \(y_p=vy\), where  \(v\) is a TBD function; without substitutin \(y\) yet, compute \(\L(vy) \).
\end{subactivity}
\begin{subactivity}
Find \(v\) from the equation \(\L(vy)=e^{3t}\).
\end{subactivity}
\begin{subactivity}
Write the general solution of \(y'-y=e^{3t}\).
\end{subactivity}
\end{activity}

\begin{activity}{10}
Find the general solution to \(y'-2y=t\).
\end{activity}


\end{applicationActivities}
