\begin{problem}{C1}
Find the general solution to
\[
y'+3y=6t+5.
\]
\end{problem}

\begin{problem}{C1}
Find the general solution to
\[
y'+4y=4.
\]
\end{problem}

\begin{problem}{C1}
Find the general solution to
\[
y'+2y=6t-1.
\]
\end{problem}

\begin{problem}{C1}
Find the general solution to
\[
y'-y=e^t.
\]
\end{problem}

\begin{problem}{C1}
Find the general solution to
\[
y'+y=e^t.
\]
\end{problem}

\begin{problem}{C1}
Find the general solution to
\[
y'-y=e^{-t}.
\]
\end{problem}

\begin{problem}{C1}
Find the general solution to
\[
y'+y=e^{-t}.
\]
\end{problem}

\begin{problem}{C1}
Find the general solution to
\[
y'+3y=10e^{-3t}\sin(t).
\]
\end{problem}

\begin{problem}{C1}
Find the general solution to
\[
y'+2y=10e^{-2t}\sin(t).
\]
\end{problem}

\begin{problem}{C1}
Find the general solution to
\[
y'+2y=5e^{-2t}\sin(t).
\]
\end{problem}

\begin{problem}{C1}
Find the general solution to
\[
y'+3y=10e^{-3t}\cos(t).
\]
\end{problem}

\begin{problem}{C1}
Find the general solution to
\[
y'+2y=10e^{-2t}\cos(t).
\]
\end{problem}

\begin{problem}{C1}
Find the general solution to
\[
y'+2y=5e^{-2t}\cos(t).
\]
\end{problem}
