\begin{problem}{C5}
Find the solution to
\[
y'' + 2y' + y = 0 
\]
when \(y(0)=0\) and \(y'(0)=2\).
\end{problem}

\begin{problem}{C5}
Find the solution to
\[
y'' + 2y' + y = 0 
\]
when \(y(0)=2\) and \(y'(0)=0\).
\end{problem}

\begin{problem}{C5}
Find the solution to
\[
y'' + 2y' - 8y = 0
\]
when \(y(0)=3\) and \(y'(0)=-6\).
\end{problem}

\begin{problem}{C5}
Find the solution to
\[
y'' + 4y' + 3y = 0
\]
when \(y(0)=1\) and \(y'(0)=5\).
\end{problem}

\begin{problem}{C5}
Find the solution to
\[
y'' + 2y' - 3y = 0
\]
when \(y(0)=5\) and \(y'(0)=1\).
\end{problem}

\begin{problem}{C5}
Find the solution to
\[
y'' + 2y' - 3y = 0
\]
when \(y(0)=2\) and \(y'(0)=2\).
\end{problem}

\begin{problem}{C5}
Find the solution to
\[
y'' - 2y' - 3y = 0
\]
when \(y(0)=2\) and \(y'(0)=2\).
\end{problem}

\begin{problem}{C5}
Find the solution to
\[
y'' + 4y' + 4y = 0
\]
when \(y(0)=1\) and \(y'(0)=3\).
\end{problem}

\begin{problem}{C5}
Find the solution to
\[
y'' - 4y' + 4y = 0
\]
when \(y(0)=1\) and \(y'(0)=3\).
\end{problem}

\begin{problem}{C5}
Find the solution to
\[
y'' + 4y' + 4y = 0
\]
when \(y(0)=3\) and \(y'(0)=1\).
\end{problem}

\begin{problem}{C5}
Find the solution to
\[
y'' - 4y' + 4y = 0
\]
when \(y(0)=3\) and \(y'(0)=1\).
\end{problem}

\begin{problem}{C5}
Find the solution to
\[
y'' + 5y' + 6y = 0
\]
when \(y(0)=3\) and \(y'(0)=1\).
\end{problem}

\begin{problem}{C5}
Find the solution to
\[
y'' + 5y' + 6y = 0
\]
when \(y(0)=1\) and \(y'(0)=2\).
\end{problem}

