\begin{problem}{D1}
Demonstrate directly from the definition that \[\L\{u(t-1)\}(s)=\frac{e^{-s}}{s}.\]
\end{problem}

\begin{problem}{D1}
Demonstrate directly from the definition that \[\L\{u(t-5)\}(s)=\frac{e^{-5s}}{s}.\]
\end{problem}

\begin{problem}{D1}
Demonstrate directly from the definition that \[\L\{\delta(t-3)\}(s)=e^{-3s}.\]
\end{problem}

\begin{problem}{D1}
Demonstrate directly from the definition that \[\L\{\delta(t-2)\}(s)=e^{-2s}.\]
\end{problem}

\begin{problem}{D1}
Demonstrate directly from the definition that \[\L\{e^{3t}\}(s)=\frac{1}{s-3}.\]
\end{problem}

\begin{problem}{D1}
Demonstrate directly from the definition that \[\L\{e^{-2t}\}(s)=\frac{1}{s+2}.\]
\end{problem}

\begin{problem}{D1}
Demonstrate directly from the definition that \[\L\{\delta(t-4)+e^t\}(s)=e^{-4s}+\frac{1}{s-1}.\]
\end{problem}

\begin{problem}{D1}
Demonstrate directly from the definition that \[\L\{\delta(t)+u(t-5)\}(s)=1+\frac{e^{-5s}}{s}.\]
\end{problem}

\begin{problem}{D1}
Demonstrate directly from the definition that \[\L\{1+e^{t}\}(s)=\frac{1}{s}+\frac{1}{s-1}.\]
\end{problem}
